coq/api2coq.v
@@ -15,224 +15,307 @@ Require Import utils.
 Instance StrDec : EqDec := {| eq_dec := string_dec |}.
 Instance NatDec : EqDec := {| eq_dec := Coq.Arith.PeanoNat.Nat.eq_dec |}.
 
-Module ML2Coq (Sg: MLSignature).
-Module Import Cervino := MLCervino(Sg).
+Section ML2Coq.
+Variable mdl : mlModel.
 
-Definition mlSorts2Sort : SortT := asFinite (mlSorts Sg.sg).
-Definition mlSort2Sort (s: mlSort) (h: List.In s (mlSorts Sg.sg)) : mlSorts2Sort :=
+Definition mlSorts2Sort : SortT := asFinite (mlSorts mdl).
+Definition mlSort2Sort (s: mlSort) (h: List.In s (mlSorts mdl)) : mlSorts2Sort :=
  exist _ s h.
 
 Instance mlVariableDec: @EqDec mlVariable.
 Proof.
   split; repeat intro.
   destruct x as [v1 h1]; destruct y as [v2 h2].
-  destruct (string_dec v1 v2); [left|right].
+  destruct (string_dec v1 v2).
   subst v2.
-  f_equal.
-  apply proof_irrelevance.
-  apply proof_irrelevance.
-
-  intro.
-  injection H; clear H; intro.
-  apply (n H).
+  destruct (string_dec h1 h2).
+  subst h2.
+  left; reflexivity.
+  right; intro.
+  injection H; intros; subst.
+  apply n; reflexivity.
+  right; intro.
+  injection H; clear H; intros.
+  apply (n H0).
 Defined.
 
 Instance mlConstantDec: @EqDec mlConstant.
 Proof.
   split; repeat intro.
   destruct x as [v1 h1]; destruct y as [v2 h2].
-  destruct (string_dec v1 v2); [left|right].
+  destruct (string_dec v1 v2).
   subst v2.
-  f_equal.
-  apply proof_irrelevance.
-  apply proof_irrelevance.
-  intro.
-  injection H; clear H; intro.
-  apply (n H).
+  destruct (string_dec h1 h2).
+  subst h2.
+  left; reflexivity.
+  right; intro.
+  injection H; intros; subst.
+  apply n; reflexivity.
+  right; intro.
+  injection H; clear H; intros.
+  apply (n H0).
 Defined.
 
 Instance mlRelationDec: @EqDec mlRelation.
 Proof.
   split; repeat intro.
   destruct x as [v1 h1]; destruct y as [v2 h2].
-  destruct (string_dec v1 v2); [left|right].
+  destruct (string_dec v1 v2).
   subst v2.
-  f_equal.
-  apply proof_irrelevance.
-  apply proof_irrelevance.
-  intro.
-  injection H; clear H; intro.
-  apply (n H).
+  destruct (list_eq_dec string_dec h1 h2).
+  subst h2.
+  left; reflexivity.
+  right; intro.
+  injection H; intros; subst.
+  apply n; reflexivity.
+  right; intro.
+  injection H; clear H; intros.
+  apply (n H0).
 Defined.
 
-(*
-Definition mlRelDec : EqDec (T := mlRelation).
-Proof.
-  split; repeat intro.
-  destruct x as [n1 a1 l1]; destruct y as [n2 a2 l2].
-  destruct (string_dec n1 n2).
-  subst n2; left.
-Defined.
-
-Definition mlRels2Rels : EqDec (T:=StrDec) :=
-  (List.map mlRelName (mlConstants srcSig))).
-*)
-
-Definition coqSig : Sig := {|
+Program Definition coqSig : Sig := {|
   Sort := mlSorts2Sort;
-  variable s := asFinite (mlVariables (proj1_sig s));
-  constant s := asFinite (mlConstants (proj1_sig s));
-  predicate := asFinite mlRelations;
+  variable s := asFinite (mlVariables mdl (proj1_sig s));
+  constant s := asFinite (mlConstants mdl (proj1_sig s));
+  predicate := asFinite (mlRelations mdl);
   pr_arity p := List.length (mlRelArity (proj1_sig p));
-  pr_args p i := 
-    mlSort2Sort (fnth (mlRelArity (proj1_sig p)) i)
-                  (mlRwf Sg.sg (mlRelName (proj1_sig p)) 
-                                  _
-                                  (mlRelationWF _)
-                                  (fnth (mlRelArity (proj1_sig p)) i)
-                                  (fnth_In _ i))
+  pr_args p i := exist _ (fnth (mlRelArity (proj1_sig p)) i) _
 |}.
+Next Obligation.
+  destruct p as [r h]; simpl in *.
+  apply (mlSortOfRel mdl r h).
+  apply fnth_In.
+Defined.
 
-Definition mlSortOfVar v: Sort (Sig:=coqSig) :=
-  (mlSort2Sort (mlVarSort v)
-    (mlVwf Sg.sg (mlVarName v) (mlVarSort v) (mlVariableWF _) )).
+Definition mlSortOfVar v h: Sort (Sig:=coqSig) :=
+  (mlSort2Sort (mlVarSort v) (mlSortOfVar mdl v h)).
 
-Definition mlSortOfCst v: Sort (Sig:=coqSig) :=
-  (mlSort2Sort (mlCstSort v)
-    (mlCwf Sg.sg (mlCstName v) (mlCstSort v) (mlConstantWF _) )).
+Definition mlSortOfCst v h: Sort (Sig:=coqSig) :=
+  (mlSort2Sort (mlCstSort v) (mlSortOfCst mdl v h)).
 
-Definition mlSortOfTerm t: Sort (Sig:=coqSig) := 
-  match t with
-    MLVar v => mlSortOfVar v
-  | MLCst c => mlSortOfCst c
+Program Definition mlSortOfTerm t: List.incl (mlTermIds t) (mlModelIds mdl) -> Sort (Sig:=coqSig) := 
+  match t return List.incl (mlTermIds t) (mlModelIds mdl) -> _ with
+    MLVar v => fun h => mlSortOfVar v _
+  | MLCst c => fun h => mlSortOfCst c _
   end.
+Next Obligation.
+  generalize (h (MLV v)); clear h; intro h.
+  assert (In (MLV v) (mlVarIds v)) by (unfold mlVarIds; simpl; tauto).
+  apply h in H; clear h.
+  unfold mlAllVariables.
+  apply (imap_filter_In_intro _ _ isMLVarDec (mlModelIds mdl)
+   (fun (v0 : mlIdent) (h1 : isMLVar v0) (_ : In v0 (mlModelIds mdl))
+      => getMLVar v0 h1) (MLV v) I H).
+Qed.
+Next Obligation.
+  generalize (h (MLC c)); clear h; intro h.
+  assert (In (MLC c) (mlCstIds c)) by (unfold mlCstIds; simpl; tauto).
+  apply h in H; clear h.
+  unfold mlAllConstants.
+  apply (imap_filter_In_intro _ _ isMLCstDec (mlModelIds mdl)
+   (fun (v0 : mlIdent) (h1 : isMLCst v0) (_ : In v0 (mlModelIds mdl))
+      => getMLCst v0 h1) (MLC c) I H).
+Qed.
 
-Lemma mlSortOfTerm_mlSort2Sort: forall t i,
-  mlSortOfTerm t = mlSort2Sort (mlTermSort t) i.
+Lemma mlSortOfTerm_mlSort2Sort: forall t h i,
+  mlSortOfTerm t h = mlSort2Sort (mlTermSort t) i.
 Proof.
   intros.
   destruct t; simpl.
-  destruct v as [v h1 h2].
+  destruct v as [v h1].
   unfold mlTermSort, mlSortOfVar, mlSort2Sort in *; simpl in *.
   f_equal.
   apply proof_irrelevance.
 
-  destruct c as [c h1 h2].
+  destruct c as [c h1].
   unfold mlTermSort, mlSortOfCst, mlSort2Sort in *; simpl in *.
   f_equal.
   apply proof_irrelevance.
 Qed.
 
-Program Definition mlVar2Var (v: mlVariable): variable (Sig:=coqSig) (mlSortOfVar v) :=
+Program Definition mlVar2Var (v: mlVariable) h: variable (Sig:=coqSig) (mlSortOfVar v h) :=
   exist _ v _.
 Next Obligation.
   unfold mlVariables.
   apply filter_In.
-  split.
-  unfold mlAllVariables.
-  set (f v h1 h2 := {| mlVarName := v; mlVar_dcl := h1; mlVar_in := h2 |}).
-  assert (v = f (mlVarName v) (mlVar_dcl v) (mlVar_in v)). 
-  destruct v; simpl; reflexivity.
-  rewrite H.
-  apply imap_filter_In_intro.
+  split; auto.
   destruct (string_dec (mlVarSort v) (mlVarSort v)); tauto.
 Qed.
 
-Program Definition mlCst2Cst (c: mlConstant): constant (Sig:=coqSig) (mlSortOfCst c) :=
+Program Definition mlCst2Cst (c: mlConstant) h: constant (Sig:=coqSig) (mlSortOfCst c h) :=
   exist _ c _.
 Next Obligation.
   unfold mlConstants.
   apply filter_In.
-  split.
-  unfold mlAllConstants.
-  set (f v h1 h2 := {| mlCstName := v; mlCst_dcl := h1; mlCst_in := h2 |}).
-  assert (c = f (mlCstName c) (mlCst_dcl c) (mlCst_in c)). 
-  destruct c; simpl; reflexivity.
-  rewrite H.
-  apply imap_filter_In_intro.
+  split; auto.
   destruct (string_dec (mlCstSort c) (mlCstSort c)); tauto.
 Qed.
 
-Definition mlTerm2Term t : term coqSig (mlSortOfTerm t) :=
-  match t return term coqSig (mlSortOfTerm t) with
-    MLVar v => Var coqSig _ (mlVar2Var v)
-  | MLCst c => Cst coqSig _ (mlCst2Cst c)
+Definition mlTerm2Term t: forall h, term coqSig (mlSortOfTerm t h) :=
+  match t return forall h, term coqSig (mlSortOfTerm t h) with
+    MLVar v => fun h => Var coqSig _ (mlVar2Var v (mlSortOfTerm_obligation_1 v h))
+  | MLCst c => fun h => Cst coqSig _ (mlCst2Cst c (mlSortOfTerm_obligation_2 c h))
   end.
 
-Program Definition mlRelation2Pred p : predicate (Sig:=coqSig) :=
-  exist _ p _.
+Definition mlRelation2Pred p (h: List.In p (mlRelations mdl)): predicate (Sig:=coqSig) :=
+  exist _ p h.
+
+Program Definition mlLiteral2Literal l:  List.incl (mlLitIds l) (mlModelIds mdl) -> literal coqSig :=
+  match l return List.incl(mlLitIds l) (mlModelIds mdl) -> literal coqSig with
+    MLPApp x p al => fun h =>
+      let r := {| mlRelName := p; mlRelArity := List.map mlTermSort al |} in
+      PApp coqSig x (mlRelation2Pred r _) 
+        (fun i => mlTerm2Term (fnth al i) _)
+  end.
 Next Obligation.
+  revert h; set (r:={| mlRelName := p; mlRelArity := map mlTermSort al |}); intros.
   unfold mlRelations.
-  set (f v h1 h2 := {| mlRelName := v; mlRel_dcl := h1; mlRel_in := h2 |}).
-  assert (p = f (mlRelName p) (mlRel_dcl p) (mlRel_in p)). 
-  destruct p; simpl; reflexivity.
-  rewrite H.
-  apply imap_filter_In_intro.
+  unfold mlRelIds in h.
+  generalize (h (MLR r) (or_introl eq_refl)); clear h; intro h.
+  apply (imap_filter_In_intro _ _ isMLRelDec (mlModelIds mdl)
+   (fun (v0 : mlIdent) (h1 : isMLRel v0) (_ : In v0 (mlModelIds mdl))
+      => getMLRel v0 h1) (MLR r) I h).
 Qed.
-
-Program Definition mlLiteral2Literal l : literal coqSig :=
-  match l with
-    MLPApp x p al h => PApp coqSig x (mlRelation2Pred p) 
-      (fun i => mlTerm2Term (fnth al i))
-  end.
 Next Obligation.
-  rewrite h.
   apply map_length.
 Qed.
 Next Obligation.
-  generalize ((mlRwf Sg.sg (mlRelName p) (mlRelArity p) (mlRelationWF p)
-     (fnth (mlRelArity p) i) (fnth_In (mlRelArity p) i))); intro.
-  generalize (mlLiteral2Literal_obligation_1 p al h); intro.
+  generalize (mlLiteral2Literal_obligation_2 x p al h).
+  generalize (mlLiteral2Literal_obligation_1 x p al h); intros.
+  apply incl_cons_inv in h; apply proj2 in h.
+  apply incl_app_inv in h; apply proj2 in h.
+  revert h; apply incl_tran.
   unfold mlRelation2Pred in e; simpl in e.
-  unfold isMLLit in h.
-  revert i i0 e; rewrite h; intros; clear h p x.
-  revert i0; rewrite (fnth_map mlTermSort al i); intro.
-  revert i i0; generalize (map_length mlTermSort al); rewrite e; simpl; intros.
-  rewrite <-mlSortOfTerm_mlSort2Sort.
-  rewrite (proof_irrelevance _ e0 eq_refl); simpl; auto.
+  revert i; rewrite e; intro; simpl.
+  apply incl_concat_r_intro with (i := (rew [Fin.t] (eq_sym (map_length mlTermIds al)) in i)).
+  rewrite fnth_map.
+  generalize (map_length mlTermIds al); intro.
+  revert i i0 e; rewrite e0; intros; simpl.
+  apply incl_refl.
+Qed.
+Next Obligation.
+  generalize (mlLiteral2Literal_obligation_3 x p al h i).
+  generalize (mlLiteral2Literal_obligation_2 x p al h).
+  generalize (mlLiteral2Literal_obligation_1 x p al h); intros.
+  simpl in e.
+  generalize (mlSortOfRel mdl {| mlRelName := p; mlRelArity := map mlTermSort al |} i0
+     (fnth (map mlTermSort al) i) (fnth_In (map mlTermSort al) i)); intro.
+  simpl in i1.
+  revert i2; rewrite fnth_map; intros.
+  revert i2; generalize (map_length mlTermSort al); intros.
+  revert i2; rewrite (proof_irrelevance _ e0 e); clear e0; intro.
+  change (fun H => Fin.t H) with Fin.t in *.
+  revert i1 i2; generalize (fnth al (rew [Fin.t] e in i)); intros.
+  rewrite mlSortOfTerm_mlSort2Sort with (i:=i2).
+  reflexivity.
 Qed.
 
-Program Definition mlAtom2Atom a : atom coqSig :=
-  match a with
-  | MLLiteral l => Literal coqSig (mlLiteral2Literal l)
-  | MLNLiteral l => NLiteral coqSig (mlLiteral2Literal l)
-  | MLEq s t1 t2 h1 h2 => Eq coqSig (mlSort2Sort s _) (mlTerm2Term t1) (mlTerm2Term t2)
-  | MLNEq s t1 t2 h1 h2 => NEq coqSig (mlSort2Sort s _)  (mlTerm2Term t1) (mlTerm2Term t2)
+Lemma mlTermSortInIds: forall t, In (MLS (mlTermSort t)) (mlTermIds t).
+Proof.
+  intros.
+  destruct t; simpl; tauto.
+Qed.
+
+Lemma mlTermIn2mlTermSortIn: forall t,
+  incl (mlTermIds t) (mlModelIds mdl) -> In (mlTermSort t) (mlSorts mdl).
+Proof.
+  intros.
+  generalize (mlTermSortInIds t); intro.
+  apply H in H0; clear H.
+  apply (imap_filter_In_intro _ _ isMLSortDec (mlModelIds mdl)
+   (fun (v0 : mlIdent) (h1 : isMLSort v0) (_ : In v0 (mlModelIds mdl))
+      => getMLSort v0 h1) (MLS _) I H0).  
+Qed.
+
+Program Definition mlAtom2Atom a : List.incl (mlAtomIds a) (mlModelIds mdl) -> formula coqSig :=
+  match a return List.incl (mlAtomIds a) (mlModelIds mdl) -> formula coqSig with
+  | MLLiteral l => fun h => Atom _ (Literal coqSig (mlLiteral2Literal l h))
+  | MLNLiteral l => fun h => Atom _ (NLiteral coqSig (mlLiteral2Literal l h))
+  | MLEq t1 t2 => fun h => let (h1,h2) := incl_app_inv _ _ h in
+    match (string_dec (mlTermSort t1) (mlTermSort t2)) with
+      left e => Atom coqSig (Eq coqSig (mlSortOfTerm t1 _) (mlTerm2Term t1 _) (mlTerm2Term t2 _))
+    | right _ => FFalse coqSig
+    end
+  | MLNEq t1 t2 => fun h => let (h1,h2) := incl_app_inv _ _ h in
+    match (string_dec (mlTermSort t1) (mlTermSort t2)) with
+      left e => Atom coqSig (NEq coqSig (mlSortOfTerm t1 _) (mlTerm2Term t1 _) (mlTerm2Term t2 _))
+    | right _ => FTrue coqSig
+    end
   end.
 Next Obligation.
-  apply mlTwf.
-Defined.
+  rewrite mlSortOfTerm_mlSort2Sort with (i:=mlTermIn2mlTermSortIn _ h1).
+  rewrite mlSortOfTerm_mlSort2Sort with (i:=mlTermIn2mlTermSortIn _ h2).
+  generalize (mlTermIn2mlTermSortIn t1 h1); rewrite e; intro.
+  f_equal; apply proof_irrelevance.
+Qed.
 Next Obligation.
-  apply mlSortOfTerm_mlSort2Sort.
-Defined.
-Next Obligation.
-  generalize (mlAtom2Atom_obligation_1 (mlTermSort t1) t1 t2 eq_refl h2).
-  rewrite <-h2.
-  apply mlSortOfTerm_mlSort2Sort.
-Defined.
-Next Obligation.
-  apply mlTwf.
-Defined.
-Next Obligation.
-  apply mlSortOfTerm_mlSort2Sort.
-Defined.
-Next Obligation.
-  generalize (mlAtom2Atom_obligation_4 (mlTermSort t1) t1 t2 eq_refl h2).
-  rewrite <-h2.
-  apply mlSortOfTerm_mlSort2Sort.
-Defined.
+  rewrite mlSortOfTerm_mlSort2Sort with (i:=mlTermIn2mlTermSortIn _ h1).
+  rewrite mlSortOfTerm_mlSort2Sort with (i:=mlTermIn2mlTermSortIn _ h2).
+  generalize (mlTermIn2mlTermSortIn t1 h1); rewrite e; intro.
+  f_equal; apply proof_irrelevance.
+Qed.
 
-Fixpoint mlFormula2formula f: formula coqSig := 
-  match f with
-    MLFTrue => FTrue coqSig
-  | MLFFalse => FFalse coqSig
-  | MLAtom a => Atom coqSig (mlAtom2Atom a)
-  | MLAnd f1 f2 => And coqSig (mlFormula2formula f1) (mlFormula2formula f2)
-  | MLOr f1 f2 => Or coqSig (mlFormula2formula f1) (mlFormula2formula f2)
-  | MLEx v b => Ex coqSig _ (mlVar2Var v) (mlFormula2formula b)
-  | MLAll v b => Ex coqSig _ (mlVar2Var v) (mlFormula2formula b)
-  | MLF f' => F coqSig (mlFormula2formula f')
-  | MLG f' => G coqSig (mlFormula2formula f')
+Lemma  mlEx_Var_In: forall {v b},
+  incl (mlFormulaIds (MLEx v b)) (mlModelIds mdl) ->
+    In v (mlAllVariables mdl).
+Proof.
+  simpl; intros.
+  apply incl_cons_inv in H; apply proj2 in H.
+  apply incl_cons_inv in H; apply proj1 in H.
+  unfold mlAllVariables.
+  apply (imap_filter_In_intro _ _ isMLVarDec (mlModelIds mdl)
+   (fun (v0 : mlIdent) (h1 : isMLVar v0) (_ : In v0 (mlModelIds mdl))
+      => getMLVar v0 h1) (MLV _) I H).
+Qed.
+
+Lemma  mlEx_bdy_incl: forall {v b},
+  incl (mlFormulaIds (MLEx v b)) (mlModelIds mdl) ->
+    incl (mlFormulaIds b) (mlModelIds mdl).
+Proof.
+  simpl; intros.
+  apply incl_cons_inv in H; apply proj2 in H.
+  apply incl_cons_inv in H; apply proj2 in H.
+  apply H.
+Qed.
+
+Lemma  mlAll_Var_In: forall {v b},
+  incl (mlFormulaIds (MLAll v b)) (mlModelIds mdl) ->
+    In v (mlAllVariables mdl).
+Proof.
+  simpl; intros.
+  apply incl_cons_inv in H; apply proj2 in H.
+  apply incl_cons_inv in H; apply proj1 in H.
+  unfold mlAllVariables.
+  apply (imap_filter_In_intro _ _ isMLVarDec (mlModelIds mdl)
+   (fun (v0 : mlIdent) (h1 : isMLVar v0) (_ : In v0 (mlModelIds mdl))
+      => getMLVar v0 h1) (MLV _) I H).
+Qed.
+
+Lemma  mlAll_bdy_incl: forall {v b},
+  incl (mlFormulaIds (MLAll v b)) (mlModelIds mdl) ->
+    incl (mlFormulaIds b) (mlModelIds mdl).
+Proof.
+  simpl; intros.
+  apply incl_cons_inv in H; apply proj2 in H.
+  apply incl_cons_inv in H; apply proj2 in H.
+  apply H.
+Qed.
+
+Fixpoint mlFormula2formula f: List.incl (mlFormulaIds f) (mlModelIds mdl) -> formula coqSig := 
+  match f return List.incl (mlFormulaIds f) (mlModelIds mdl) -> formula coqSig with
+    MLFTrue => fun h => FTrue coqSig
+  | MLFFalse => fun h => FFalse coqSig
+  | MLAtom a => mlAtom2Atom a
+  | MLAnd f1 f2 => fun h => 
+    let (h1,h2) := incl_app_inv _ _ h in
+    And coqSig (mlFormula2formula f1 h1) (mlFormula2formula f2 h2)
+  | MLOr f1 f2 => fun h => 
+    let (h1,h2) := incl_app_inv _ _ h in
+    Or coqSig (mlFormula2formula f1 h1) (mlFormula2formula f2 h2)
+  | MLEx v b => fun h => Ex coqSig _ (mlVar2Var v (mlEx_Var_In h)) (mlFormula2formula b (mlEx_bdy_incl h))
+  | MLAll v b => fun h => All coqSig _ (mlVar2Var v (mlAll_Var_In h)) (mlFormula2formula b (mlAll_bdy_incl h))
+  | MLF f' => fun h => F coqSig (mlFormula2formula f' h)
+  | MLG f' => fun h => G coqSig (mlFormula2formula f' h)
   end.
 
 End ML2Coq.
