coq/closure.v
@@ -1,6 +1,9 @@
 
 Require Import Eqdep_dec.
 Require Import Fin.
+Import EqNotations.
+Require Import FunctionalExtensionality.
+Require Import ProofIrrelevance.
 
 Require Import foltl.
 Require Import dec.
@@ -10,18 +13,41 @@ Require Import varset.
 Require Import vars.
 Require Import fosem.
 
+Ltac psemTac :=
+    match goal with
+      H:psem _ _ ?sa |- psem _ _ ?sa' => assert (sa' = sa) as ae;
+          try (rewrite ae; assumption); (apply functional_extensionality_dep; intros)
+    end.
+    
+
+Inductive Closure {T} (R: T -> T -> Prop): T -> T -> Prop :=
+  Cl0: forall d1 d2, d1=d2 -> Closure R d1 d2
+| ClS: forall d1 d2 d3, Closure R d1 d2 -> R d2 d3 -> Closure R d1 d3.
+
 Section Closure.
   Context {Ts: Type} {Tv: Ts->Type} {Tc: Ts->Type} {Tp: Type}.
-  Variable Sg: @Sig Ts Tv Tc Tp.
-  Variable D: Dom Sg.
+  Variable srcSg: @Sig Ts Tv Tc Tp.
+  Variable D: Dom srcSg.
   Variable s: Sort.
-  Variable itp: Interp D.
-  Variable BinItp: ssem s -> ssem s -> Prop.
+  Variable srcItp: Interp D.
+  Variable Succ: predicate.
+  Variable Succ': predicate.
+  Variable SuccAr: pr_arity Succ = 2.
+  Variable SuccAr': pr_arity Succ' = 2.
+  Variable SuccArgs: forall i, pr_args Succ i = s.
+  Variable SuccArgs': forall i, pr_args Succ' i = s.
+  Variable Succ_stb: forall t1 t2 a, psem Succ t1 a <-> psem Succ t2 a.
+  
+  Definition SuccSem t (x y: ssem s) :=
+    psem Succ t (fun i => match i with F1 => rew [ssem] (eq_sym (SuccArgs i)) in x | _ => rew [ssem] (eq_sym (SuccArgs i)) in y end).
 
-  Inductive Closure: ssem s -> ssem s -> Prop :=
-    Cl0: forall d1 d2, d1=d2 -> Closure d1 d2
-  | ClS: forall d1 d2 d3, Closure d1 d2 -> BinItp d2 d3 -> Closure d1 d3.
-
+  Definition SuccSem' t (x y: ssem s) :=
+    psem Succ' t (fun i => match i with F1 => rew [ssem] (eq_sym (SuccArgs' i)) in x | _ => rew [ssem] (eq_sym (SuccArgs' i)) in y end).
+  
+  Definition ClosureSem := forall t x y, SuccSem' t x y <-> Closure (SuccSem t) x y.
+  
+  Variable SuccSem_cls': ClosureSem.
+  
   Inductive AuxVars := X1 | X2 | Z1 | Z2.
   Program Definition AuxVarsDec: @EqDec AuxVars := {| eq_dec := _ |}.
   Next Obligation.
@@ -33,87 +59,165 @@ Section Closure.
   Next Obligation.
     destruct x; tauto.
   Qed.
-    
-  Inductive BinPreds := Succ | Succ'.
-  Program Definition BinPredsDec: @EqDec BinPreds := {| eq_dec := _ |}.
-  Next Obligation.
-    repeat intro.
-    decide equality.
-  Qed.
-  Definition BinPredsSet: SV.set BinPredsDec := (cons Succ (cons Succ' nil)).
-  Program Definition BinPredsFin: Finite := {| fin_set := BinPredsSet |}.
-  Next Obligation.
-    destruct x; tauto.
-  Qed.
   
-  Definition epredicate := (SumDec BinPredsDec predicate).
-
-  Definition epr_arity (p': epredicate) := match p' with inl p => 2 | inr p => pr_arity p end.
-  Definition epr_args p': Fin.t (epr_arity p') -> _ :=
-    match p' return Fin.t (epr_arity p') -> _ with 
-      inl p => fun i => s
-    | inr p => fun i => pr_args p i 
-    end.
-  
-  Definition srcSg : Sig := {|
-    Sort := Sort (Sig:=Sg);
-    constant := constant;
-    variable := variable;
-    predicate := epredicate;
-    pr_arity := epr_arity;
-    pr_args := epr_args;
-  |}.
-
   Definition dstVarT s' (e: {s'=s}+{s'<>s}): Type := if e then AuxVars + (variable s') else variable s'.
 
   Definition dstSg : Sig := {|
-    Sort := Sort (Sig:=Sg);
+    Sort := Sort (Sig:=srcSg);
     variable := fun s' => if eq_dec s' s as e return @VariableT (dstVarT s' e) then (SumFin AuxVarsFin (variable s')) else variable s';
     constant := constant;
-    predicate := epredicate;
-    pr_arity := epr_arity;
-    pr_args := epr_args;
+    predicate := predicate;
+    pr_arity := pr_arity;
+    pr_args := pr_args;
   |}.
   
-  Program Definition srcD: Dom srcSg := {| ssem := ssem (Dom:=D); neDom := neDom (Dom:=D) |}.
-
   Program Definition dstD: Dom dstSg := {| ssem := ssem (Dom:=D); neDom := neDom (Dom:=D) |}.
   
-  Program Definition srcItp : Interp srcD := {|
-    csem s c := csem (Interp:=itp) c;
-    psem p t := match (p: predicate (Sig:=srcSg)) as p0 return 
-      (forall i : Fin.t (epr_arity p0), ssem (epr_args p0 i)) -> Prop with 
-      inl np =>
-        match np return (Fin.t 2 -> ssem s) -> _ with 
-          Succ => fun a => BinItp (a F1) (a (FS F1))
-        | Succ' => fun a => Closure (a F1) (a (FS F1))
-        end
-    | inr p => psem p t
-    end
-  |}.
+  Program Definition dstItp : Interp dstD := {| csem s c := csem (Interp:=srcItp) c; psem := psem (Interp:=srcItp) |}.
 
-  Program Definition dstItp : Interp dstD := {|
-    csem s c := csem (Interp:=itp) c;
-    psem p t := match (p: predicate (Sig:=dstSg)) as p0 return 
-      (forall i : Fin.t (epr_arity p0), ssem (epr_args p0 i)) -> Prop with 
-      inl np =>
-        match np return (Fin.t 2 -> ssem s) -> _ with 
-          Succ => fun a => BinItp (a F1) (a (FS F1))
-        | Succ' => fun a => Closure (a F1) (a (FS F1))
-        end
-    | inr p => psem p t
-    end
-  |}.
+  Definition tfrVar {s'} (v: variable (Sig:=srcSg) s') : variable (Sig:=dstSg) s'.
+  Proof.
+    unfold variable; simpl.
+    destruct (eq_dec s' s); simpl.
+    exact (inr v).
+    exact v.
+  Defined.
+  
+  Definition tfrTerm {s} (tm: term srcSg s): term dstSg s :=
+  match tm return term dstSg s with
+    Cst _ _ c => Cst dstSg _ c
+  | Var _ _ v => Var dstSg _ (tfrVar v)
+  end.
+  
+  Definition tfrLiteral (l: literal srcSg): literal dstSg :=
+  match l with
+    PApp _ x r args => PApp dstSg x r (fun i => tfrTerm (args i))
+  end.
+  
+  Definition tfrAtom (a: atom srcSg): atom dstSg :=
+  match a with
+    Literal _ l => Literal dstSg (tfrLiteral l)
+  | NLiteral _ l => NLiteral dstSg (tfrLiteral l)
+  | Eq _ s t1 t2 => Eq dstSg s (tfrTerm t1) (tfrTerm t2)
+  | NEq _ s t1 t2 => NEq dstSg s (tfrTerm t1) (tfrTerm t2)
+  end.
+  
+  Fixpoint tfrFormula (f: formula srcSg): formula dstSg :=
+  match f with
+  | FTrue _ => FTrue dstSg
+  | FFalse _ => FFalse dstSg
+  | Atom _ a => Atom dstSg (tfrAtom a)
+  | And _ f1 f2 => And dstSg (tfrFormula f1) (tfrFormula f2)
+  | Or _ f1 f2 => Or dstSg (tfrFormula f1) (tfrFormula f2)
+  | Ex _ s v f => Ex dstSg s (tfrVar v) (tfrFormula f)
+  | All _ s v f => All dstSg s (tfrVar v) (tfrFormula f)
+  | F _ f => F dstSg (tfrFormula f)
+  | G _ f => G dstSg (tfrFormula f)
+  end.
+
+  Definition tfrEnv (env: Env srcSg D) : Env dstSg dstD.
+  Proof.
+    intro s'.
+    unfold variable; simpl.
+    unfold dstVarT in *; simpl.
+    destruct (@eq_dec Ts (@Sort Ts Tv Tc Tp srcSg) s' s); intro v.
+    destruct v.
+    exact (neDom _).
+    exact (env _ e0).
+    exact (env _ v).
+  Defined.
+
+  Lemma tfr_env_sem: forall env s' v, env s' v = tfrEnv env s' (tfrVar v).
+  Proof.
+    unfold tfrEnv, tfrVar; simpl; intros.
+    destruct (eq_dec s' s); auto.
+  Qed.
+
+  Lemma tfr_addEnv: forall env s' (v: variable (Sig:=srcSg) s') d,
+    add dstSg (tfrVar v) d (tfrEnv env) = tfrEnv (add srcSg v d env).
+  Proof.
+    intros.
+    apply functional_extensionality_dep; intro s''.
+    apply functional_extensionality; intro w.
+    destruct (eq_dec s'' s').
+    subst.
+    destruct (eq_dec (tfrVar v) w); auto.
+    subst w.
+    rewrite <-tfr_env_sem.
+    do 2 rewrite add_eq; now auto.
+    rewrite add_ne.
+    revert w n; unfold tfrEnv, tfrVar, add; simpl.
+    destruct (eq_dec s' s); simpl; intros; auto.
+    subst s'.
+    destruct w; simpl; auto.
+    destruct (eq_dec s s); try tauto.
+    rewrite (proof_irrelevance _ e0 eq_refl).
+    destruct (eq_dec v e); auto.
+    subst v; tauto.
+    destruct (eq_dec s' s'); try tauto.
+    rewrite (proof_irrelevance _ e eq_refl).
+    destruct (eq_dec v w); auto; tauto.
+    apply n.
+    
+    rewrite add_ne2.
+    revert w n; unfold tfrEnv, tfrVar, dstVarT, add; simpl.
+    destruct (@eq_dec Ts (@Sort Ts Tv Tc Tp srcSg) s'' s); simpl; intros; auto.
+    destruct w; simpl; auto.
+    subst s''.
+    destruct (eq_dec s' s); try (subst s'; tauto); auto.
+    destruct (eq_dec s' s''); try (subst s''; tauto); auto.
+    intro; apply n.
+    injection H; intros; auto.
+  Qed.
+
+  Lemma tfr_tm_sem: forall env s' (tm: term srcSg s'), tm_sem srcSg (Itp:=srcItp) env tm = tm_sem dstSg (Itp:=dstItp) (tfrEnv env) (tfrTerm tm).
+  Proof.
+    intros.
+    destruct tm; simpl; auto.
+    apply tfr_env_sem.
+  Qed.
+  
+  Lemma tfr_lt_sem: forall env l t, lt_sem srcSg (Itp:=srcItp) env l t <-> lt_sem dstSg (Itp:=dstItp) (tfrEnv env) (tfrLiteral l) t.
+  Proof.
+    intros.
+    destruct l; simpl.
+    split; intro; psemTac.
+    symmetry; apply tfr_tm_sem.
+    apply tfr_tm_sem.
+  Qed.
+  
+  Lemma tfr_at_sem: forall env a t, at_sem srcSg (Itp:=srcItp) env a t <-> at_sem dstSg (Itp:=dstItp) (tfrEnv env) (tfrAtom a) t.
+  Proof.
+    intros.
+    destruct a; simpl.
+    apply tfr_lt_sem.
+    apply not_iff_compat; apply tfr_lt_sem.
+    do 2 rewrite tfr_tm_sem; reflexivity.
+    apply not_iff_compat; do 2 rewrite tfr_tm_sem; reflexivity.
+  Qed.
+    
+  Lemma tfr_sem: forall env f t, fm_sem srcSg (Itp:=srcItp) env f t <-> fm_sem dstSg (Itp:=dstItp) (tfrEnv env) (tfrFormula f) t.
+  Proof.
+    intros.
+    revert env t; induction f; intros; simpl; try tauto.
+    apply tfr_at_sem.
+    rewrite IHf1; rewrite IHf2; reflexivity.
+    rewrite IHf1; rewrite IHf2; reflexivity.
+    setoid_rewrite tfr_addEnv; setoid_rewrite IHf; reflexivity.
+    setoid_rewrite tfr_addEnv; setoid_rewrite IHf; reflexivity.
+    setoid_rewrite IHf; reflexivity.
+    setoid_rewrite IHf; reflexivity.
+  Qed.
   
   Definition at_Succ (x1 x2: term dstSg s): formula dstSg :=
     Atom dstSg (Literal dstSg
-     (PApp dstSg 0 (inl Succ)
-        (fun i : Fin.t 2 => match i with F1 => x1 | _ => x2 end))).
+     (PApp dstSg 0 Succ
+        (fun i => rew eq_sym (SuccArgs i) in match rew SuccAr in i with F1 => x1 | _ => x2 end))).
 
   Definition at_Succ' (x1 x2: term dstSg s): formula dstSg :=
     Atom dstSg (Literal dstSg
-     (PApp dstSg 0 (inl Succ')
-        (fun i : Fin.t 2 => match i with F1 => x1 | _ => x2 end))).
+     (PApp dstSg 0 Succ'
+        (fun i => rew eq_sym (SuccArgs' i) in match rew SuccAr' in i with F1 => x1 | _ => x2 end))).
 
   Definition var (v: AuxVars): variable (Sig:=dstSg) s.
   Proof.
@@ -132,62 +236,173 @@ Section Closure.
     exfalso; clear H; tauto.
   Qed.
   
-  Definition unary (P: formula dstSg) (x: variable (Sig:=dstSg) s) :=
-    vsIn dstSg x (free dstSg P) /\ 
-    vsSubset dstSg (free dstSg P) (vsSing dstSg x).
-    
-  Definition subst (x y: variable (Sig:=dstSg) s) (P: formula dstSg) :=
-    Ex dstSg s x (And dstSg (Atom dstSg (Eq dstSg s (Var dstSg s y) (Var dstSg s x))) P).
-
-  Notation "'[' x ':=' y ']'" := (subst x y).
+  Definition unary `{Sg: Sig} {s} (P: formula Sg) (x: variable (Sig:=Sg) s) :=
+    vsIn Sg x (free Sg P) /\ 
+    vsSubset Sg (free Sg P) (vsSing Sg x).
   
-  Lemma subst_sem:
+  Lemma unary_dec: forall `{Sg: Sig} {s} (P: formula Sg) (x: variable (Sig:=Sg) s), {unary P x} + {not (unary P x)}.
+  Proof.
+    intros.
+    apply (AndDec {| dc_dec := vsIn_dec Sg x (free Sg P) |}
+                     {| dc_dec := vsSubset_dec Sg (free Sg P) (vsSing Sg x) |}).
+  Qed.
+  
+  Lemma tfr_free: forall (P: formula srcSg) s' (w: variable s'),
+    vsIn srcSg w (free srcSg P) <-> vsIn dstSg (tfrVar w) (free dstSg (tfrFormula P)).
+  Proof.
+    clear D srcItp SuccSem_cls' Succ_stb.
+  Admitted.
+  
+  Lemma tfr_aux: forall (P: formula srcSg) x,
+    not (vsIn dstSg (var x) (free dstSg (tfrFormula P))).
+  Proof.
+    clear D srcItp SuccSem_cls' Succ_stb.
+  Admitted.
+  
+  Lemma unary_tfr: forall (P: formula srcSg) (v: variable s), unary P v -> unary (tfrFormula P) (tfrVar v).
+  Proof.
+    intros.
+    destruct H.
+    split; intros.
+    rewrite <-tfr_free; auto.
+    
+    intros s' w h.
+    apply (vsSing_intro_eq dstSg).
+    rewrite tfr_free in H.
+    generalize (vsSubsetSing_r srcSg (free srcSg P) H0 ); clear H0; intro.
+    setoid_rewrite tfr_free in H0.
+    assert (vsIn dstSg w (free dstSg (tfrFormula P))) by (apply h); clear h.
+    generalize (tfr_aux P).
+    revert H H1 H0; generalize (free dstSg (tfrFormula P)) as F; intros.
+    revert H H1 H0 H2; generalize (@vsIn _ _ _ _ dstSg).
+    intros.
+    set (P0F s v := P0 s v F).
+    assert (forall s v, P0F s v = P0 s v F) by (intros; reflexivity).
+    rewrite <-H3 in *.
+    setoid_rewrite <-H3 in H0.
+    setoid_rewrite <-H3 in H2.
+    clear H3; clearbody P0F; clear P0 F.
+    generalize (H0 s); intro.
+    generalize (H0 s'); intro.
+    clear H0.
+    destruct (eq_dec s' s).
+    subst s'.
+    clear H4.
+    revert H H1 H2 H3; generalize (P0F s) as PFs; clear P0F; intros.
+    assert (forall w : variable s, PFs (tfrVar w) -> w = v).
+      intros.
+      apply H3 in H0.
+      apply inj_pair2_eq_dec in H0; try apply eq_dec; now auto.
+    clear H3.
+    assert (w = tfrVar v).
+    revert v w PFs H H1 H2 H0.
+    unfold tfrVar, variable, dstSg, dstVarT, var; simpl.
+    destruct (eq_dec s s); simpl; intros.
+    destruct w; auto.
+    apply H2 in H1; tauto.
+    
+    apply H0 in H1; subst e0; tauto.
+    apply H0 in H1; now auto.
+    subst w; reflexivity.
+    
+    exfalso.
+    assert (forall w, P0F s' (tfrVar w) -> False).
+      intros.
+      apply H4 in H0.
+      injection H0; intros; tauto.
+    clear H4.
+    assert (forall w : variable s, P0F s (tfrVar w) -> w = v).
+      intros.
+      apply H3 in H4.
+      apply inj_pair2_eq_dec in H4; try apply eq_dec; auto.
+    clear H3.
+    revert w H H1 H2 H0 H4.
+    generalize (P0F s) as PF; generalize (P0F s') as PF'; clear P0F.
+    unfold tfrVar, variable, dstSg, dstVarT, var; simpl.
+    
+    destruct (@eq_dec Ts (@Sort Ts Tv Tc Tp srcSg) s' s); try tauto.
+    clear n0.
+    destruct (@eq_dec Ts (@Sort Ts Tv Tc Tp srcSg) s s); auto; try tauto; intros.
+    apply H0 in H1; tauto.
+  Qed.
+  
+  Definition vsubst (x y: variable (Sig:=dstSg) s) (P: formula dstSg) :=
+    subst dstSg x (Var dstSg s y) P.
+
+  Notation "'[' x ':=' y ']'" := (vsubst x y).
+  
+  Lemma vsubst_sem:
     forall (f: formula dstSg) (itp: Interp dstD) (env1 env2: Env dstSg dstD) t (x y: variable (Sig:=dstSg) s), 
     unary f x -> env1 s x = env2 s y -> x <> y ->
       fm_sem dstSg (Itp:=itp) env1 f t <-> fm_sem dstSg (Itp:=itp) env2 ([x:=y] f) t.
   Proof.
     intros.
-    unfold subst.
-    rewrite Ex_sem.
-    setoid_rewrite And_sem.
-    simpl.
-    setoid_rewrite add_eq.
-    split; intros.
-    exists (env2 s y); split; auto.
-    rewrite add_upd; auto.
-    rewrite <-H0.
-    revert H2; apply fm_sem_equiv; intros.
-    apply H in H2.
-    apply (vsSing_elim dstSg) in H2.
-    injection H2; intros; subst s0.
+    apply subst_sem; intros; auto.
+    unfold unary in H.
+    apply (proj2 H) in H2.
+    exfalso; apply H3; clear H3.
+    symmetry.
+    apply vsSing_elim; auto.
+    simpl; intro.
+    apply vsSing_elim in H2.
+    injection H2; intros; subst.
     apply inj_pair2_eq_dec in H3; try apply eq_dec.
-    subst v.
-    rewrite add_eq; reflexivity.
-    
-    destruct H2 as [d [h1 h2]].
-    revert h2; apply fm_sem_equiv; intros.
-    apply H in H2.
-    apply (vsSing_elim dstSg) in H2.
-    injection H2; intros; subst s0.
-    apply inj_pair2_eq_dec in H3; try apply eq_dec.
-    subst v.
-    rewrite add_eq.
-    rewrite add_ne in h1; auto.
-    subst d; auto.
+    tauto.
   Qed.
   
-  Definition Propagates (P: formula dstSg) (fp: unary P (var X1)) :=
-   All dstSg _ (var X1) (All dstSg _ (var X2) (G dstSg
-    (Imp dstSg (And dstSg P (at_Succ (Var dstSg s (var X1)) (Var dstSg s (var X2))))
-          (F dstSg ([var X1 := var X2] P ))))).
+  Definition Propagates (P: formula dstSg) v (fp: unary P v) :=
+   All dstSg _ v (All dstSg _ (var X2) (G dstSg
+    (Imp dstSg (And dstSg P (at_Succ (Var dstSg s v) (Var dstSg s (var X2))))
+          (F dstSg ([v := var X2] P ))))).
 
-  Definition AbsClosure (P: formula dstSg) (fp: unary P (var X1)) :=
-    All dstSg _ (var Z1) (Imp dstSg  (And dstSg ([var X1 := var Z1] P ) (Propagates P fp))
-                       (All dstSg _ (var Z2) (Imp dstSg (at_Succ' (Var dstSg s (var Z1)) (Var dstSg s (var Z2))) (F dstSg ([var X1 := var Z2] P ))))).
+  Definition AbsClosure (P: formula dstSg) v (fp: unary P v) :=
+    All dstSg _ (var Z1) (Imp dstSg  (And dstSg ([v := var Z1] P ) (Propagates P v fp))
+                       (All dstSg _ (var Z2) (Imp dstSg (at_Succ' (Var dstSg s (var Z1)) (Var dstSg s (var Z2))) (F dstSg ([v := var Z2] P ))))).
 
-  Theorem AbsClosureOK: forall (P: formula dstSg) (fp: unary P (var X1)),
-    forall (v: variable (Sig:=dstSg) s), 
-      forall (env: Env dstSg dstD) t, fm_sem (Itp:=dstItp) dstSg env (AbsClosure P fp) t.
+  Lemma SuccSem_equ: forall env t t1 t2, fm_sem (Itp:=dstItp) dstSg env (at_Succ t1 t2) t <-> SuccSem t (tm_sem (Itp:=dstItp) dstSg env t1) (tm_sem (Itp:=dstItp) dstSg env t2).
+   Proof.
+    intros.
+    unfold SuccSem; simpl.
+    clear SuccSem_cls' SuccArgs' SuccAr'.
+    generalize (psem Succ t) as ps.
+    revert SuccArgs; generalize (pr_args Succ) as pa.
+    rewrite SuccAr; clear SuccAr; intros.
+    assert (pa = fun i => s).
+      apply functional_extensionality; apply SuccArgs.
+    subst pa; simpl.
+    assert (SuccArgs = fun i => eq_refl).
+      apply functional_extensionality; intro.
+      apply proof_irrelevance.
+    subst SuccArgs; simpl.
+    match goal with |- ps ?f1 <-> ps ?f2 => assert (f1 = f2) end.
+    apply functional_extensionality; intro i.
+    destruct i; simpl; auto.
+    rewrite H; tauto.
+   Qed.
+
+   Lemma SuccSem_equ': forall env t t1 t2, fm_sem (Itp:=dstItp) dstSg env (at_Succ' t1 t2) t <-> SuccSem' t (tm_sem (Itp:=dstItp) dstSg env t1) (tm_sem (Itp:=dstItp) dstSg env t2).
+   Proof.
+    intros.
+    unfold SuccSem'; simpl.
+    clear SuccSem_cls' SuccArgs SuccAr Succ_stb Succ.
+    generalize (psem Succ' t) as ps.
+    revert SuccArgs'; generalize (pr_args Succ') as pa.
+    rewrite SuccAr'; clear SuccAr'; intros.
+    assert (pa = fun i => s).
+      apply functional_extensionality; apply SuccArgs'.
+    subst pa; simpl.
+    assert (SuccArgs' = fun i => eq_refl).
+      apply functional_extensionality; intro.
+      apply proof_irrelevance.
+    subst SuccArgs'; simpl.
+    match goal with |- ps ?f1 <-> ps ?f2 => assert (f1 = f2) end.
+    apply functional_extensionality; intro i.
+    destruct i; simpl; auto.
+    rewrite H; tauto.
+   Qed.
+
+  Theorem AbsClosureOK: forall (P: formula dstSg) v (fp: unary P (tfrVar v)),
+      forall (env: Env dstSg dstD) t, fm_sem (Itp:=dstItp) dstSg env (AbsClosure P (tfrVar v) fp) t.
   Proof.
     intros.
     unfold AbsClosure.
@@ -196,7 +411,6 @@ Section Closure.
     apply And_sem in H; destruct H.
     apply All_sem; intro.
     apply Imp_sem; intro.
-    simpl in H1.
     assert ((add dstSg (var Z2) d0 (add dstSg (var Z1) d env) s
           (var Z1)) = d).
       rewrite add_ne.
@@ -206,21 +420,26 @@ Section Closure.
     assert ((add dstSg (var Z2) d0 (add dstSg (var Z1) d env) s
           (var Z2)) = d0).
       apply add_eq.
+    apply SuccSem_equ' in H1.
+    simpl in H1.
     rewrite H2,H3 in H1; clear H2 H3.
     
+    apply SuccSem_cls' in H1.
     induction H1.
     subst d2.
     exists t; split; auto.
     clear H0.
     simpl in d1.
-    rewrite <-subst_sem with (env1:=add dstSg (var X1) (d1: ssem (Dom:=dstD) s) env) in H; auto.
-    rewrite <-subst_sem with (env1:=add dstSg (var X1) (d1: ssem (Dom:=dstD) s) env); auto.
+    rewrite <-vsubst_sem with (env1:=add dstSg (tfrVar v) (d1: ssem (Dom:=dstD) s) env) in H; auto.
+    rewrite <-vsubst_sem with (env1:=add dstSg (tfrVar v) (d1: ssem (Dom:=dstD) s) env); auto.
     do 2 rewrite add_eq; now auto.
     intro.
-    apply var_inj in H0; discriminate.
+    unfold tfrVar, var in H0; simpl in H0.
+    destruct (eq_dec s s); auto; try tauto; discriminate.
     do 2 rewrite add_eq; now auto.
     intro.
-    apply var_inj in H0; discriminate.
+    unfold tfrVar, var in H0; simpl in H0.
+    destruct (eq_dec s s); auto; try tauto; discriminate.
         
     generalize (IHClosure H H0); clear IHClosure H; intro H.
     destruct H as [t' [h1 h2]].
@@ -232,7 +451,7 @@ Section Closure.
     rewrite Imp_sem in H0.
     match goal with H0: ?p -> _ |- _ => assert p as h; [clear H0 | apply H0 in h; clear H0] end.
     apply And_sem; split.
-    rewrite <-subst_sem with (env1:=add dstSg (var X1) (d2: ssem (Dom:=dstD) s) env) in h2; auto.
+    rewrite <-vsubst_sem with (env1:=add dstSg (tfrVar v) (d2: ssem (Dom:=dstD) s) env) in h2; auto.
     revert h2; apply fm_sem_equiv; intros; auto.
     apply fp in H; apply (vsSing_elim dstSg) in H.
     injection H; intros; subst s0.
@@ -240,25 +459,80 @@ Section Closure.
     repeat rewrite add_eq.
     rewrite add_ne; try (intro diff; apply var_inj in diff; discriminate).
     rewrite add_eq; now auto.
+    unfold tfrVar, var; simpl.
+    destruct (eq_dec s s); auto; try tauto; discriminate.
     repeat rewrite add_eq; now auto.
-    intro diff; apply var_inj in diff; discriminate.
+    unfold tfrVar, var; simpl.
+    destruct (eq_dec s s); auto; try tauto; discriminate.
 
     simpl.
+    apply Succ_stb with (t2:=t).
+    apply SuccSem_equ; simpl.  
+    
     rewrite add_eq.
     rewrite add_ne; try (intro diff; apply var_inj in diff; discriminate).
     rewrite add_eq.
     apply H2.
 
+    unfold tfrVar, var; simpl.
+    destruct (eq_dec s s); auto; try tauto; discriminate.
+
     rewrite F_sem in h; destruct h as [t'' [h h']].
     exists t''; split.
     apply Arith.Le.le_trans with t'; now auto.
-    rewrite <-subst_sem with (env1:=add dstSg (var X1) (d3: ssem (Dom:=dstD) s) env) in h'; auto.
-    rewrite <-subst_sem with (env1:=add dstSg (var X1) (d3: ssem (Dom:=dstD) s) env); auto.
+    rewrite <-vsubst_sem with (env1:=add dstSg (tfrVar v) (d3: ssem (Dom:=dstD) s) env) in h'; auto.
+    rewrite <-vsubst_sem with (env1:=add dstSg (tfrVar v) (d3: ssem (Dom:=dstD) s) env); auto.
     repeat rewrite add_eq; auto.
-    intro diff; apply var_inj in diff; discriminate.
+    unfold tfrVar, var; simpl.
+    destruct (eq_dec s s); auto; try tauto; discriminate.
     repeat rewrite add_eq; auto.
-    intro diff; apply var_inj in diff; discriminate.
+    unfold tfrVar, var; simpl.
+    destruct (eq_dec s s); auto; try tauto; discriminate.
   Qed.
 End Closure.
 
-  
+Record ClosureSpec `(srcSg : Sig) (s: Sort) (Succ Succ' : predicate) (P: formula srcSg) (v: variable s):= {
+  cs_ar: pr_arity Succ = 2;
+  cs_ar': pr_arity Succ' = 2;
+  cs_prf: forall i : Fin.t (pr_arity Succ), pr_args Succ i = s;
+  cs_prf': forall i : Fin.t (pr_arity Succ'), pr_args Succ' i = s;
+  cs_one: unary P v;
+}.
+Arguments cs_ar [_ _ _ _ _ _ _ _ _ _] _.
+Arguments cs_ar' [_ _ _ _ _ _ _ _ _ _] _.
+Arguments cs_prf [_ _ _ _ _ _ _ _ _ _] _.
+Arguments cs_prf' [_ _ _ _ _ _ _ _ _ _] _.
+Arguments cs_one [_ _ _ _ _ _ _ _ _ _] _.
+
+Lemma ClosureSpec_dec: forall `{srcSg : Sig} {s: Sort} (Succ Succ' : predicate) (P: formula srcSg) (v: variable s),
+  {ClosureSpec srcSg s Succ Succ' P v} + { not (ClosureSpec srcSg s Succ Succ' P v)}.
+Proof.
+  intros.
+  destruct (Peano_dec.eq_nat_dec (pr_arity Succ) 2); [idtac | right; intro cs; destruct cs; tauto].
+  destruct (Peano_dec.eq_nat_dec (pr_arity Succ') 2); [idtac | right; intro cs; destruct cs; tauto].
+  destruct (all_dec (fun i => isEq (pr_args Succ i) s)); [idtac | destruct s0 as [i h]; simpl in h; right; intro cs; destruct cs; auto].
+  destruct (all_dec (fun i => isEq (pr_args Succ' i) s)); [idtac | destruct s0 as [i h]; simpl in h; right; intro cs; destruct cs; auto].
+  destruct (unary_dec P v).
+  left; split; simpl in *; intros; auto.
+  right; intro cs; destruct cs; auto.
+Qed.
+
+Definition cs_sem `{srcSg: Sig} {s} {Succ Succ'} {P} {v} (cs: ClosureSpec srcSg s Succ Succ' P v) {D: Dom srcSg} (itp: Interp D) : Prop :=
+  ClosureSem srcSg D s itp Succ Succ' (cs_prf cs) (cs_prf' cs) /\
+  forall t1 t2 a, psem Succ t1 a <-> psem Succ t2 a.
+
+Definition absClosure`{srcSg: Sig} {s} {Succ Succ'} {P} {v} (cs: ClosureSpec srcSg s Succ Succ' P v) :=
+  AbsClosure srcSg s Succ Succ' (cs_ar cs) (cs_ar' cs) (cs_prf cs) (cs_prf' cs) (tfrFormula srcSg s P) (tfrVar srcSg s v) (unary_tfr srcSg _  _ _ (cs_ar cs) (cs_ar' cs) (cs_prf cs) (cs_prf' cs) P v (cs_one cs)).
+
+Lemma elim_cs: forall `(srcSg: Sig) s Succ Succ' P v (cs: ClosureSpec srcSg s Succ Succ' P v) (f: formula srcSg) {D: Dom srcSg} (itp: Interp D) env t,
+  (cs_sem cs itp /\ fm_sem srcSg (Itp:=itp) env f t) -> 
+    fm_sem (dstSg srcSg s) (Itp:=dstItp srcSg D s itp) (tfrEnv srcSg D s env) (And _ (absClosure cs) (tfrFormula srcSg s f)) t.
+Proof.
+  intros.
+  destruct H.
+  apply And_sem; split.
+  apply AbsClosureOK; intros; auto.
+  apply (proj2 H).
+  apply (proj1 H).
+  apply tfr_sem; auto.
+Qed.
