coq/transfo.v
@@ -1,22 +1,18 @@
+Require Import ProofIrrelevance.
+Import  EqNotations.
+Require Import List.
+
 Require Import api.
 Require Import api2coq.
-Require Import abstraction.
 Require Import foltl.
 Require Import set.
 Require Import finite.
+Require abstraction.
+Require closure.
 
-(***
-Record mlSignedFormula := { (* A REVOIR: changement de signature *)
-  mlSfForm : mlFormula;
-}.
-
-Definition mlTransform (m: mlModel) (chk: mlCheck) : option mlSignedFormula.
-Admitted.
-***)
-Module Transfo (Sg: MLSignature).
-  Module Import AsCoq := ML2Coq(Sg).
-  Import Cervino.
-
+Section Transfo.
+  Variable mdl: mlModel.
+  
   Definition mlConj l := List.fold_right (fun a r => MLAnd a r) MLFTrue l.
 
   Definition mlDisj l := List.fold_right (fun a r => MLOr a r) MLFFalse l.
@@ -26,27 +22,154 @@ Module Transfo (Sg: MLSignature).
   Definition mlEvtSem e :=
     mlArgs2Ex (mlEvArgs e) (mlEvBody e).
 
-  Definition mdl_sem (m: mlModel) :=
-    let axms := mlConj (mlAxioms m) in
-    let evts := mlDisj (List.map mlEvtSem (mlEvents m)) in
-    MLAnd axms evts.
+  Definition mlAxmSem (m: mlModel) := mlConj (mlAxioms m).
 
-  Definition applyTEA (m: mlModel) (chk: mlCheck) :=
-    let f := mlChkBody chk in
-    let cf := mlFormula2formula f in
-    let fv s := vars.free coqSig cf s in 
-    match isExAll_dec coqSig cf with
+  Lemma mlDisjIds: forall l F, (forall f, List.In f l -> List.incl (mlFormulaIds f) F)
+    -> List.incl (mlFormulaIds (mlDisj l)) F.
+  Proof.
+    induction l; simpl; intros; auto.
+    repeat intro.
+    destruct H0.
+    apply List.incl_app.
+    apply H; tauto.
+    apply IHl; intros.
+    apply H; tauto.
+  Qed.
+
+  Lemma mlConjIds: forall l F, (forall f, List.In f l -> List.incl (mlFormulaIds f) F)
+    -> List.incl (mlFormulaIds (mlConj l)) F.
+  Proof.
+    induction l; simpl; intros; auto.
+    repeat intro.
+    destruct H0.
+    apply List.incl_app.
+    apply H; tauto.
+    apply IHl; intros.
+    apply H; tauto.
+  Qed.
+
+  Lemma mlArgs2ExIds: forall l f,
+    List.incl (mlFormulaIds (mlArgs2Ex l f)) (List.map (fun a => MLS (mlVarSort a)) l ++ List.map MLV l ++ mlFormulaIds f).
+  Proof.
+    induction l; simpl; intros; auto.
+    apply incl_refl.
+    apply incl_cons; simpl; try tauto.
+    apply incl_cons; simpl.
+    right.
+    rewrite in_app_iff; right; simpl; tauto.
+    specialize IHl with f.
+    apply incl_tran with (map (fun a : mlVariable => MLS (mlVarSort a)) l ++
+         map MLV l ++ mlFormulaIds f); auto; clear IHl.
+    change (MLS (mlVarSort a)
+       :: map (fun a0 : mlVariable => MLS (mlVarSort a0)) l ++
+      MLV a :: map MLV l ++ mlFormulaIds f) with
+      ((MLS (mlVarSort a)::nil)++
+       (map (fun a0 : mlVariable => MLS (mlVarSort a0)) l) ++
+      MLV a :: map MLV l ++ mlFormulaIds f).
+    apply incl_appr.
+    apply incl_app_app.
+    apply incl_refl.
+    change (MLV a :: map MLV l ++ mlFormulaIds f) with
+      ((MLV a :: nil) ++ map MLV l ++ mlFormulaIds f).
+    apply incl_appr.
+    apply incl_refl.
+  Qed.
+
+  Program Definition applyTEA :=
+    let chk := mlCheckWith mdl in
+    let f := mlDisj (List.map mlEvtSem (mlEvents mdl)) in
+    let cf := mlFormula2formula mdl f _ in
+    let fv s := vars.free (coqSig mdl) cf s in 
+    let g := MLAnd (mlAxmSem mdl) (mlChkBody chk) in
+    let cg := mlFormula2formula mdl g _ in
+    match isExAll_dec (coqSig mdl) cf with
       left exAll => 
         match all_dec (fun s => SV.emptyDec (fv s)) with
-          inl ise => Some (abstract_ExAll coqSig cf exAll ise)
+          inl ise => Some (abstraction.abstract_G_EAf_and_g (coqSig mdl) cf cg exAll ise)
         | inr _ => None
         end
     | right _ => None
     end.
+  Next Obligation.
+    apply mlDisjIds; intros.
+    apply List.in_map_iff in H.
+    destruct H as [x [h1 h2]].
+    unfold mlModelIds.
+    apply List.incl_appr.
+    apply List.incl_appl.
+    apply utils.in_fnth in h2.
+    destruct h2 as [i h2].
+    apply utils.in_concat_map_intro.
+    exists i.
+    subst f; subst x.
+    unfold mlEvtSem.
+    generalize (utils.fnth (mlEvents mdl) i); intro f.
+    generalize (mlArgs2ExIds (mlEvArgs f) (mlEvBody f)); intro.
+    apply incl_tran with
+      (map (fun a : mlVariable => MLS (mlVarSort a)) (mlEvArgs f) ++
+        map MLV (mlEvArgs f) ++ mlFormulaIds (mlEvBody f)); auto.
+    clear H.
+    rewrite <-map_map.
+    unfold mlEventIds.
+    apply incl_app.
+    apply List.incl_appr.
+    apply List.incl_appl; apply List.incl_refl.
+    
+    apply incl_app.
+    apply List.incl_appl; apply List.incl_refl.
+    apply List.incl_appr; apply List.incl_appr; apply List.incl_refl.
+  Qed.
+  Next Obligation.
+    unfold mlModelIds.
+    apply incl_app.
+    apply incl_appl.
+    unfold mlAxmSem.
+    apply (mlConjIds (mlAxioms mdl)); intros.
+    apply utils.in_concat_map_intro.
+    apply utils.in_fnth in H; destruct H as [i H]; subst f.
+    exists i; apply incl_refl.
 
-  Definition mlTransform (m: mlModel) (chk: mlCheck) :=
+    admit.
+  Admitted.
+
+  Definition applyTEA_Sg :=
+    abstraction.dstSig (coqSig mdl)
+       (quantifiers.getExF
+         (mlFormula2formula mdl
+           (mlDisj (map mlEvtSem (mlEvents mdl)))
+           applyTEA_obligation_1)).
+
+  Program Definition applyTTC (r: mlRelation) hr (v: mlVariable) hv (P: mlFormula) hP:
+    option (formula (closure.dstSg (coqSig mdl) (mlSortOfVar mdl v hv))) :=
+    let cr := mlRelation2Pred mdl r hr in
+    let cls := mlClosures mdl in
+    let lp := utils.imap cls (fun p h => 
+      (mlRelation2Pred mdl (mlBase p) _, mlRelation2Pred mdl (mlTC p) _)) in 
+    match dec.assoc cr lp with
+      None => None
+    | Some r' =>
+      let cf: formula (coqSig mdl) := mlFormula2formula mdl P hP in
+      let cv := mlVar2Var mdl v _ in
+      match closure.ClosureSpec_dec (srcSg := coqSig mdl) cr r' cf cv with
+        left cs => Some (closure.absClosure cs)
+      | right _ => None
+      end
+    end.
+  Next Obligation.
+    unfold mlRelations.
+    unfold mlModelIds.
+  Admitted.
+  Next Obligation.
+  Admitted.
+  
+  Definition applyTTCSig v hv :=
+    closure.dstSg (coqSig mdl) (mlSortOfVar mdl v hv).
+  
+  Definition mlTransform : option ( :=
+    let chk := mlCheckWith mdl in
     match mlChkUsing chk with
-      TEA => applyTEA m chk
+      TEA => applyTEA
+    | TTC r v P => applyTTC r _ v _ P _
     | _ => None
     end.
 
